Makefile
@@ -2,9 +2,12 @@
 
 coqc Coqlib.v Integers.v SHA256.v ;
 coqc Axioms.v Extensionality.v Coqlib2.v common_lemmas.v functional_prog.v ;
-coqc pure_lemmas.v sha_padding_lemmas.v hmac_pure_lemmas.v hmac_common_lemmas.v ;
-coqc XorCorrespondence.v Bruteforce.v ByteBitRelations.v HMAC_common_defs.v ;
-coqc HMAC_functional_prog.v HMAC_functional_prog_Z.v HMAC_spec_pad.v 
-     HMAC_spec_concat.v HMAC_spec_list.v HMAC_spec_abstract.v 
+coqc XorCorrespondence.v # Takes a long time, skip after compiling once
+
+coqc pure_lemmas.v sha_padding_lemmas.v hmac_pure_lemmas.v ;
+coqc HMAC_functional_prog.v HMAC_functional_prog_Z.v hmac_common_lemmas.v ;
+coqc Bruteforce.v ByteBitRelations.v ;
+coqc HMAC_common_defs.v HMAC_spec_pad.v HMAC_spec_concat.v HMAC_spec_list.v
+     HMAC_spec_abstract.v 
 
 
